Bugged

Eval.v
@@ -55,14 +55,23 @@ Module EVAL <: EVALTYPE.
       remember (RLIST.find (0, ref null) compFirst vals) as fres; destruct fres; symmetry in Heqfres;
       apply RLIST.findRelEq in Heqfres; try constructor; auto.
       remember (RLIST.get n vals) as gres; destruct gres; symmetry in Heqgres; apply RLIST.getRelEq in Heqgres.
-      destruct t.
+      destruct t. econstructor. eapply Heqfres. eapply Heqgres.
+      eapply someNoneEvalRegRel. eapply Heqfres. apply Heqgres.
+      remember (RLIST.find ((S n), ref null) compFirst vals) as fres; destruct fres; symmetry in Heqfres;
+      apply RLIST.findRelEq in Heqfres; try constructor; auto.
+      remember (RLIST.get n0 vals) as gres; destruct gres; symmetry in Heqgres; apply RLIST.getRelEq in Heqgres.
+      destruct t. econstructor. eapply Heqfres. eapply Heqgres.
+      eapply someNoneEvalRegRel. eapply Heqfres. apply Heqgres.
+    inversion H; subst; destruct n; simpl; try reflexivity;
+      try (apply RLIST.findRelEq in H0; rewrite H0; try reflexivity; apply RLIST.getRelEq in H1; rewrite H1; reflexivity).
+  Qed.
 
-  Fixpoint evalLhs (exp:lhs) (st:DVMState) : @Option Val :=
+  Definition evalLhs (exp:lhs) (st:DVMState) : @Option Val :=
     match exp,st with
     | (reg n),_ => evalReg n st
     | (acc n n2),dst _ h _ _ _ => match (evalReg n st) with
       | Some (ref (lRef lc)) => match (HP.get lc h),(evalReg n2 st) with
-        | Some (ar (arr n' lst)),(Some (prim (int n''))) => (VLIST.get n'' lst)
+        | Some (ar (arr n' lst)),(Some (prim p1)) => (VLIST.get (PType.toNat p1) lst)
         | _,_ => None
         end
       | _ => None
@@ -88,8 +97,149 @@ Module EVAL <: EVALTYPE.
       | None => None
       end
     | _ , _ => None
-    end
-  with evalRhs (exp:rhs) (st:DVMState) : @Option Val :=
+    end.
+
+  Inductive evalLhsRel : lhs -> DVMState -> @Option Val -> Prop :=
+    | regEvalLhsRel : forall (n:nat) (st:DVMState) (v:@Option Val), evalRegRel n st v -> evalLhsRel (reg n) st v
+    | noneFirstAccEvalLhsRel : forall (n n2:nat) (st:DVMState), evalRegRel n st None -> evalLhsRel (acc n n2) st None
+    | somePrimFirstAccEvalLhsRel : forall (n n2:nat) (p:Prim) (st:DVMState), evalRegRel n st (Some (prim p)) -> evalLhsRel (acc n n2) st None
+    | someNullFirstAccEvalLhsRel : forall (n n2:nat) (st:DVMState), evalRegRel n st (Some (ref null)) -> evalLhsRel (acc n n2) st None
+    | noneSecondAccEvalLhsRel : forall (n n2:nat) (st:DVMState), evalRegRel n2 st None -> evalLhsRel (acc n n2) st None
+    | someRefSecondAccEvalLhsRel : forall (n n2:nat) (r:Ref) (st:DVMState), evalRegRel n2 st (Some (ref r)) -> evalLhsRel (acc n n2) st None
+    | someNoneAccEvalLhsRel : forall (n n2:nat) (lc:Location) (frms:list Frame) (h:Heap) (sh:SHeap) (inb outb:Buffer),
+                              evalRegRel n (dst frms h sh inb outb) (Some (ref (lRef lc))) ->
+                              HP.getRel lc h None ->
+                              evalLhsRel (acc n n2) (dst frms h sh inb outb) None
+    | someSomeDobAccEvalLhsRel : forall (n n2:nat) (lc:Location) (object:Object) (frms:list Frame) (h:Heap) (sh:SHeap) (inb outb:Buffer),
+                              evalRegRel n (dst frms h sh inb outb) (Some (ref (lRef lc))) ->
+                              HP.getRel lc h (Some (dob object)) ->
+                              evalLhsRel (acc n n2) (dst frms h sh inb outb) None
+    | someSomeArAccEvalLhsRel : forall (n n1 n2 n':nat) (lc:Location) (p1:Prim) (frms:list Frame) (h:Heap) (sh:SHeap) (inb outb:Buffer) (v:@Option Val) (lst:list Val),
+                              evalRegRel n (dst frms h sh inb outb) (Some (ref (lRef lc))) ->
+                              HP.getRel lc h (Some (ar (arr n' lst))) ->
+                              evalRegRel n2 (dst frms h sh inb outb) (Some (prim p1)) ->
+                              PType.toNatRel p1 n1 ->
+                              VLIST.getRel n1 lst v ->
+                              evalLhsRel (acc n n2) (dst frms h sh inb outb) v
+    | noneFirstIfieldEvalLhsRel : forall (n1 n2:nat) (st:DVMState), evalRegRel n1 st None -> evalLhsRel (ifield n1 n2) st None
+    | somePrimFirstIfieldEvalLhsRel : forall (n1 n2:nat) (st:DVMState) (p1:Prim), evalRegRel n1 st (Some (prim p1)) -> evalLhsRel (ifield n1 n2) st None
+    | someNullFirstIfieldEvalLhsRel : forall (n1 n2:nat) (st:DVMState), evalRegRel n1 st (Some (ref null)) -> evalLhsRel (ifield n1 n2) st None
+    | someNoneIfieldEvalLhsRel : forall (n1 n2:nat) (lc:Location) (frms:list Frame) (h:Heap) (sh:SHeap) (inb outb:Buffer),
+                              evalRegRel n1 (dst frms h sh inb outb) (Some (ref (lRef lc))) ->
+                              HP.getRel lc h None ->
+                              evalLhsRel (ifield n1 n2) (dst frms h sh inb outb) None
+    | someArIfieldEvalLhsRel : forall (n1 n2:nat) (array:Array) (lc:Location) (frms:list Frame) (h:Heap) (sh:SHeap) (inb outb:Buffer),
+                              evalRegRel n1 (dst frms h sh inb outb) (Some (ref (lRef lc))) ->
+                              HP.getRel lc h (Some (ar array)) ->
+                              evalLhsRel (ifield n1 n2) (dst frms h sh inb outb) None
+    | someTopIfieldEvalLhsRel : forall (n1 n2:nat) (lc:Location) (frms:list Frame) (h:Heap) (sh:SHeap) (inb outb:Buffer),
+                              evalRegRel n1 (dst frms h sh inb outb) (Some (ref (lRef lc))) ->
+                              HP.getRel lc h (Some (dob topObj)) ->
+                              evalLhsRel (ifield n1 n2) (dst frms h sh inb outb) None
+    | someDobjIfieldEvalLhsRel : forall (n1 n2:nat) (lc:Location) (frms:list Frame) (h:Heap) (sh:SHeap) (inb outb:Buffer),
+                              evalRegRel n1 (dst frms h sh inb outb) (Some (ref (lRef lc))) ->
+                              HP.getRel lc h (Some (dob dobj)) ->
+                              evalLhsRel (ifield n1 n2) (dst frms h sh inb outb) None
+    | someObjNoneIfieldEvalLhsRel : forall (n1 n2 n3 n4:nat) (lc:Location) (frms:list Frame) (h:Heap) (sh:SHeap) (inb outb:Buffer) (lst:list (FieldLocation*Val)),
+                              evalRegRel n1 (dst frms h sh inb outb) (Some (ref (lRef lc))) ->
+                              HP.getRel lc h (Some (dob (obj n3 n4 lst))) ->
+                              LVLIST.findRel (n2,(ref null)) compFirst lst None ->
+                              evalLhsRel (ifield n1 n2) (dst frms h sh inb outb) None
+    | someObjSomeNoneIfieldEvalLhsRel : forall (n1 n2 n3 n4 n5:nat) (lc:Location) (frms:list Frame) (h:Heap) (sh:SHeap) (inb outb:Buffer) (lst:list (FieldLocation*Val)),
+                              evalRegRel n1 (dst frms h sh inb outb) (Some (ref (lRef lc))) ->
+                              HP.getRel lc h (Some (dob (obj n3 n4 lst))) ->
+                              LVLIST.findRel (n2,(ref null)) compFirst lst (Some n5) ->
+                              LVLIST.getRel n5 lst None ->
+                              evalLhsRel (ifield n1 n2) (dst frms h sh inb outb) None
+    | someObjSomeSomeIfieldEvalLhsRel : forall (n1 n2 n3 n4 n5 n6:nat) (lc:Location) (frms:list Frame) (h:Heap) (sh:SHeap) (inb outb:Buffer) (lst:list (FieldLocation*Val)) (v1:Val),
+                              evalRegRel n1 (dst frms h sh inb outb) (Some (ref (lRef lc))) ->
+                              HP.getRel lc h (Some (dob (obj n3 n4 lst))) ->
+                              LVLIST.findRel (n2,(ref null)) compFirst lst (Some n5) ->
+                              LVLIST.getRel n5 lst (Some (n6,v1)) ->
+                              evalLhsRel (ifield n1 n2) (dst frms h sh inb outb) (Some v1)
+    | noneSfieldEvalLhsRel : forall (n:nat) (frms:list Frame) (h:Heap) (sh:SHeap) (inb outb:Buffer),
+                              SVLIST.findRel (n,(ref null)) compFirst sh None ->
+                              evalLhsRel (sfield n) (dst frms h sh inb outb) None
+    | someNoneSfieldEvalLhsRel : forall (n n2:nat) (frms:list Frame) (h:Heap) (sh:SHeap) (inb outb:Buffer),
+                              SVLIST.findRel (n,(ref null)) compFirst sh (Some n2) ->
+                              SVLIST.getRel n2 sh None ->
+                              evalLhsRel (sfield n) (dst frms h sh inb outb) None
+    | someSomeSfieldEvalLhsRel : forall (n n2 n3:nat) (frms:list Frame) (h:Heap) (sh:SHeap) (inb outb:Buffer) (v1:Val),
+                              SVLIST.findRel (n,(ref null)) compFirst sh (Some n2) ->
+                              SVLIST.getRel n2 sh (Some (n3,v1)) ->
+                              evalLhsRel (sfield n) (dst frms h sh inb outb) (Some v1)
+    | stuckEvalLhsRel : forall (l1:lhs), evalLhsRel l1 stuck None
+    | haltEvalLhsRel : forall (l1:lhs), evalLhsRel l1 halt None.
+
+  Theorem evalLhsRelEq : forall (l1:lhs) (st:DVMState) (v1:@Option Val), evalLhs l1 st = v1 <-> evalLhsRel l1 st v1.
+  Proof.
+    split; intro.
+    destruct st; simpl in H; subst; destruct l1; simpl; try constructor; (try (destruct r; constructor)).
+    remember (evalReg r (dst frms h sh inb outb)) as eregr. destruct eregr; symmetry in Heqeregr; apply evalRegRelEq in Heqeregr; assumption.
+    remember (evalReg r (dst frms h sh inb outb)) as eregr. destruct eregr; symmetry in Heqeregr; try (apply evalRegRelEq in Heqeregr; apply noneFirstAccEvalLhsRel; assumption).
+    destruct v. eapply somePrimFirstAccEvalLhsRel. eapply evalRegRelEq. eauto.
+    destruct r1; (try (apply someNullFirstAccEvalLhsRel; apply evalRegRelEq; auto)).
+    remember (HP.get l h) as getl. destruct getl; symmetry in Heqgetl; apply HP.getRelEq in Heqgetl.
+      destruct t. destruct a.
+        remember (evalReg r0 (dst frms h sh inb outb)) as eregr0. destruct eregr0; symmetry in Heqeregr0; apply evalRegRelEq in Heqeregr0.
+          destruct v. remember (VLIST.get (PType.toNat p) l0) as get2. symmetry in Heqget2. remember (PType.toNat p) as n'. symmetry in Heqn'.
+          eapply someSomeArAccEvalLhsRel. eapply evalRegRelEq. eapply Heqeregr. eapply Heqgetl. apply Heqeregr0. eapply PType.toNatRelEq. eapply Heqn'.
+          eapply VLIST.getRelEq. assumption. eapply someRefSecondAccEvalLhsRel. eapply Heqeregr0.
+          eapply noneSecondAccEvalLhsRel. assumption. 
+          remember (evalReg r0 (dst frms h sh inb outb)) as eregr0. destruct eregr0; symmetry in Heqeregr0.
+            eapply someSomeDobAccEvalLhsRel. eapply evalRegRelEq. eapply Heqeregr. eapply Heqgetl.
+          eapply noneSecondAccEvalLhsRel. eapply evalRegRelEq. assumption.
+          eapply someNoneAccEvalLhsRel. eapply evalRegRelEq. eapply Heqeregr. assumption.
+    remember (evalReg r (dst frms h sh inb outb)) as eregr. destruct eregr; symmetry in Heqeregr; apply evalRegRelEq in Heqeregr; (try (eapply noneFirstIfieldEvalLhsRel; assumption)).
+    destruct v. eapply somePrimFirstIfieldEvalLhsRel. apply Heqeregr.
+    destruct r0. remember (HP.get l h) as getl. symmetry in Heqgetl. apply HP.getRelEq in Heqgetl. destruct getl.
+    destruct t. eapply someArIfieldEvalLhsRel. apply Heqeregr. apply Heqgetl.
+    destruct o. eapply someTopIfieldEvalLhsRel. apply Heqeregr. assumption.
+    remember (LVLIST.find (f, ref null) compFirst l0) as fres. symmetry in Heqfres. apply LVLIST.findRelEq in Heqfres.
+    destruct fres. remember (LVLIST.get n l0) as getl0. symmetry in Heqgetl0. apply LVLIST.getRelEq in Heqgetl0. destruct getl0.
+    destruct t. eapply someObjSomeSomeIfieldEvalLhsRel. eapply Heqeregr. eapply Heqgetl. eapply Heqfres. eapply Heqgetl0.
+    eapply someObjSomeNoneIfieldEvalLhsRel. eapply Heqeregr. eapply Heqgetl. eapply Heqfres. eapply Heqgetl0.
+    eapply someObjNoneIfieldEvalLhsRel. eapply Heqeregr. eapply Heqgetl. eapply Heqfres.
+    eapply someDobjIfieldEvalLhsRel. eapply Heqeregr. eapply Heqgetl.
+    eapply someNoneIfieldEvalLhsRel. eapply Heqeregr. eapply Heqgetl.
+    apply someNullFirstIfieldEvalLhsRel. assumption.
+    remember (SVLIST.find (f, ref null) compFirst sh) as fres. symmetry in Heqfres. apply SVLIST.findRelEq in Heqfres.
+    destruct fres. remember (SVLIST.get n sh) as getn. symmetry in Heqgetn. apply SVLIST.getRelEq in Heqgetn.
+    destruct getn. destruct t. eapply someSomeSfieldEvalLhsRel. eapply Heqfres. eapply Heqgetn.
+    eapply someNoneSfieldEvalLhsRel. eapply Heqfres. assumption.
+    eapply noneSfieldEvalLhsRel. assumption.
+    (* If part done *)
+    inversion H; simpl.
+      apply evalRegRelEq in H0; rewrite H0; reflexivity.
+      apply evalRegRelEq in H0; rewrite H0; destruct st; reflexivity.
+      apply evalRegRelEq in H0; rewrite H0; destruct st; reflexivity.
+      apply evalRegRelEq in H0; rewrite H0; destruct st; reflexivity.
+      apply evalRegRelEq in H0; rewrite H0; destruct st; try reflexivity. destruct (evalReg n (dst frms h sh inb outb)); destruct v; auto; destruct r; auto. destruct (HP.get l h); auto. destruct t; auto. destruct a; auto.
+      apply evalRegRelEq in H0; rewrite H0; destruct st; try reflexivity. destruct (evalReg n (dst frms h sh inb outb)); destruct v; auto; destruct r0; auto. destruct (HP.get l h); auto. destruct t; auto. destruct a; auto.
+      apply evalRegRelEq in H0; rewrite H0. eapply HP.getRelEq in H1. rewrite H1. reflexivity.
+      apply evalRegRelEq in H0; rewrite H0. eapply HP.getRelEq in H1. rewrite H1. reflexivity.
+      apply evalRegRelEq in H0; rewrite H0. eapply HP.getRelEq in H1. rewrite H1. apply evalRegRelEq in H2. rewrite H2. apply PType.toNatRelEq in H3. rewrite H3. apply VLIST.getRelEq. assumption.
+      destruct st; auto; apply evalRegRelEq in H0; rewrite H0; auto.
+      destruct st; auto; apply evalRegRelEq in H0; rewrite H0; auto.
+      destruct st; auto; apply evalRegRelEq in H0; rewrite H0; auto.
+      apply evalRegRelEq in H0; rewrite H0; auto. apply HP.getRelEq in H1. rewrite H1. reflexivity.
+      apply evalRegRelEq in H0; rewrite H0; auto. apply HP.getRelEq in H1. rewrite H1. reflexivity.
+      apply evalRegRelEq in H0; rewrite H0; auto. apply HP.getRelEq in H1. rewrite H1. reflexivity.
+      apply evalRegRelEq in H0; rewrite H0; auto. apply HP.getRelEq in H1. rewrite H1. reflexivity.
+      apply evalRegRelEq in H0; rewrite H0; auto. apply HP.getRelEq in H1. rewrite H1. apply LVLIST.findRelEq in H2. rewrite H2.
+(* ShortCuts
+      try (destruct st; simpl; reflexivity); try (apply HP.getRelEq in H1; rewrite H1; simpl; auto); try (destruct l1; simpl; reflexivity).
+      destruct st; try reflexivity. destruct (evalReg n (dst frms h sh inb outb)); destruct v; simpl; try reflexivity. destruct r; auto. destruct (HP.get l h); auto. destruct t; auto. destruct a; auto.
+      destruct st; try reflexivity. destruct (evalReg n (dst frms h sh inb outb)); destruct v; simpl; try reflexivity. destruct r0; auto. destruct (HP.get l h); auto. destruct t; auto. destruct a; auto.
+      apply evalRegRelEq in H2. rewrite H2. apply PType.toNatRelEq in H3. rewrite H3. apply VLIST.getRelEq. assumption.
+*)
+(** Bug Alert *)
+      remember (LVLIST.find (n2, ref null) (@compFirst Val) lst) as fres.
+      destruct lst. simpl. reflexivity. simpl.
+      subst; destruct (LVLIST.find (n2, ref null) compFirst lst). destruct (HP.get lc h); auto. destruct t; auto. destruct a; auto. 
+      apply evalRegRelEq in H0; rewrite H0.
+
+  Definition evalRhs (exp:rhs) (st:DVMState) : @Option Val :=
     match exp with
     | (l lhs1) => (evalLhs lhs1 st)
     | (cs cnst) => match cnst with
@@ -99,4 +249,5 @@ Module EVAL <: EVALTYPE.
       | cnull => Some (ref null)
       end
     end.
+
 End EVAL.
